wip

theories/Monads/STM/STMModels.v
@@ -30,29 +30,22 @@ Import Basics.Monads.
 
 From Coinduction Require Import all.
 
-From RelationAlgebra Require Import lattice monoid prop rel.
+From RelationAlgebra Require Import lattice monoid prop rel srel.
 
 #[local] Open Scope itree_scope.
 
-(* Universe conflict when trying to include CTree.Eq and ITree.Events.FailFacts *)
-(*
-#[local] Unset Universe Checking.
-From CTree Require Import CTree Eq.
-*)
-
-
 Section transaction_sim.
 
-Context {E F : Type -> Type} {Si Sm : Type}.
+Context {E F : Type -> Type} {Si Sm X : Type}.
 
-Context (i : E ~> stateT Sm (itree void1)).
+Context (i : E ~> stateT Sm (itree G)).
 (* i is the specification handler for shared state events *)
 
 Context (h : transactionE E ~> itree F).
 (* h takes transactions with state events E and translates them into events F
    that are interleaved with other transactions. *)
 
-Context (g : F ~> stateT Si (itree void1)).
+Context (g : F ~> stateT Si (itree H)).
 (* g translates F events into operations on the implementation state. *)
 
 Context (HS : Si -> Sm -> Prop).
@@ -62,37 +55,42 @@ Variant transaction_event :=
 | TransEvDone (s : Si)
 | TransEvRet {R} (r : R)
 | TransEvStep
+| TransEvError
 | TransEvNew {R} (t : itree E (option R))
 .
 
 Variant transaction_impl :=
-| TransImpl {R} (t : itree F (option R)).
+| TI {R} (t : itree F (option R)).
 
-Variant trans_impl_move : transaction_event -> (Si * list transaction_impl) -> (Si * list transaction_impl) -> Prop :=
+Variant transaction_move : transaction_event -> hrel (Si * list transaction_impl) (Si * list transaction_impl) :=
 | TransMoveDone (s : Si) :
-    trans_impl_move (TransEvDone s) (s, []) (s, [])
+    transaction_move (TransEvDone s) (s, []) (s, [])
 | TransMoveRet {R} (r : R) (t : itree F (option R)) s ts1 ts2 :
     t ≅ Ret (Some r) ->
-    trans_impl_move (TransEvRet r) (s, ts1 ++ [TransImpl t] ++ ts2) (s, ts1 ++ ts2)
+    transaction_move (TransEvRet r) (s, ts1 ++ [TI t] ++ ts2) (s, ts1 ++ ts2)
 | TransMoveAbort {R} (t : itree F (option R)) s ts1 ts2 :
     t ≅ Ret None ->
-    trans_impl_move TransEvStep (s, ts1 ++ [TransImpl t] ++ ts2) (s, ts1 ++ ts2)
+    transaction_move TransEvStep (s, ts1 ++ [TI t] ++ ts2) (s, ts1 ++ ts2)
 | TransMoveStep {R} (t t' : itree F (option R)) s ts1 ts2 :
     t ≅ Tau t' ->
-    trans_impl_move TransEvStep (s, ts1 ++ [TransImpl t] ++ ts2) (s, ts1 ++ [TransImpl t'] ++ ts2)
+    transaction_move TransEvStep (s, ts1 ++ [TI t] ++ ts2) (s, ts1 ++ [TI t'] ++ ts2)
 | TransMoveVis {R T} (t : itree F (option R)) (r : T) (e : F T) (k : T -> itree F (option R)) s s' ts1 ts2 :
     t ≅ Vis e k ->
-    g _ e s ≅ Ret (s', r) ->
-    trans_impl_move TransEvStep (s, ts1 ++ [TransImpl t] ++ ts2) (s', ts1 ++ [TransImpl (k r)] ++ ts2)
+    g _ e s ≈ Ret (s', r) ->
+    transaction_move TransEvStep (s, ts1 ++ [TI t] ++ ts2) (s', ts1 ++ [TI (k r)] ++ ts2)
+| TransMoveVis {R T} (t : itree F (option R)) (r : T) (e : F T) (k : T -> itree F (option R)) s s' ts1 ts2 :
+    t ≅ Vis e k ->
+    g _ e s ≈ Vis e' k' ->
+    transaction_move TransEvError (s, ts1 ++ [TI t] ++ ts2) (s', ts1 ++ [TI (k r)] ++ ts2)
 | TransMoveNewTransaction {R} (t : itree E (option R)) (s : Si) (ts : list transaction_impl) :
-    trans_impl_move (TransEvNew t) (s, ts) (s, TransImpl (h _ (Transaction t)) :: ts)
+    transaction_move (TransEvNew t) (s, ts) (s, TI (h _ (Transaction t)) :: ts)
 .
 
 Variant transaction_state : Type :=
 | Pending {R} (p : itree E (option R))
 | Committed {R} (r : R).
 
-Inductive trans_move : (Sm * list transaction_state) -> (Sm * list transaction_state) -> Prop :=
+Inductive trans_move : hrel (Sm * list transaction_state) (Sm * list transaction_state) :=
 | CommitTransaction {R} (t : itree E (option R)) (r : R) (s1 s2 : Sm) (ts1 ts2 : list transaction_state) :
     interp_state i t s1 ≈ Ret (s2, Some r) ->
     trans_move (s1, ts1 ++ [Pending t] ++ ts2) (s2, ts1 ++ [Committed r] ++ ts2)
@@ -105,137 +103,13 @@ Variant trans_response (sim : (Sm * list transaction_state) -> Prop) : transacti
 | TransResRet {R} (r : R) (s : Sm) (ts1 ts2 : list transaction_state) : sim (s, ts1 ++ ts2) -> trans_response sim (TransEvRet r) (s, ts1 ++ [Committed r] ++ ts2).
 
 Program Definition transactionalb : mon ((Si * list transaction_impl) -> (Sm * list transaction_state) -> Prop) :=
-  {| body R s1 s2 := forall ev s1', trans_impl_move ev s1 s1' -> exists s2', trans_move ^* s2 s2' /\ trans_response (R s1') ev s2' |}.
+  {| body R s1 s2 := forall ev s1', transaction_move ev s1 s1' -> exists s2', trans_move ^* s2 s2' /\ trans_response (R s1') ev s2' |}.
+Next Obligation.
+  apply H1 in H2 as [s2' [Hmoves Hresponse]].
+  exists s2'.
+  split; [assumption|].
+  destruct Hresponse; constructor; auto.
+Defined.
 
 End transaction_sim.
-
-
-
-Section example.
-
-  #[global] Instance EqDec_unit : EqDec unit eq :=
-    fun x y => match x, y with tt, tt => left eq_refl end.
-
-  Definition nats (_ : unit) : Type := nat.
-
-  Definition fib_trans (x0 x1 : TVar nats nat): itree (stmE nats) unit :=
-    v0 <- readTVar x0 ;;
-    v1 <- readTVar x1 ;;
-    writeTVar x0 v1 ;;
-    writeTVar x1 (v0 + v1).
-
-  Definition fib (n : nat) : itree (runStmE nats +' forkE) unit :=
-    '(x, y) <- atomically (
-      x <- newTVar tt 0 ;;
-      y <- newTVar tt 1 ;;
-      Ret (x, y)) ;;
-    (fix fib_ n :=
-      match n with
-      | 0 => Ret tt
-      | S n => fork (atomically (fib_trans x y)) (fib_ n)
-      end) n.
-
-  Variant result (E : Type -> Type) (A : Type) :=
-  | Val : A -> result E A
-  | NotYet : result E A
-  | Event : forall {X}, E X -> result E A.
-
-  Arguments Val {E A} (a).
-  Arguments NotYet {E A}.
-  Arguments Event {E A} {X} (e).
-
-  Definition force {E A} (n : nat) (t : itree E A) : result E A :=
-    match observe (burn n t) with
-    | RetF a => Val a
-    | TauF _ => NotYet
-    | VisF e _ => Event e
-    end.
-
-  Definition unwrap {E A} : option A -> itree E A :=
-    fun o => match o with None => ITree.spin | Some a => Ret a end.
-
-  Compute (force 178 (run_atomic_transactions (run_atomically (fib 8)))).
-  Compute (force 1000 (run_single_lock_fork (run_atomically (fib 8)))).
-  Compute (force 1874 (run_tl2_fork (run_atomically (fib 8)))).
-
-  Definition read_test : itree (runStmE nats +' forkE) unit :=
-    x <- atomically (newTVar tt 21) ;;
-    atomically (readTVar x) ;;
-    Ret tt.
-
-  Definition write_test : itree (runStmE nats +' forkE) unit :=
-    x <- atomically (newTVar tt 22) ;;
-    atomically (writeTVar x 23).
-
-  Definition inc_test : itree (runStmE nats +' forkE) unit :=
-    x <- atomically (newTVar tt 0) ;;
-    atomically (v <- readTVar x ;; writeTVar x (S v)).
-
-  Compute (force 1000 (run_tl2_fork (run_atomically read_test))).
-  Compute (force 1000 (run_tl2_fork (run_atomically write_test))).
-  Compute (force 1000 (run_tl2_fork (run_atomically inc_test))).
-
-  Definition takeMVar {K} {V : K -> Type} {A} (t : TVar V (option A)) : itree (stmE V) A :=
-    v <- readTVar t ;;
-    match v with
-    | None => retry
-    | Some a => writeTVar t None ;; Ret a
-    end.
-
-  Definition putMVar {K} {V : K -> Type} {A} (t : TVar V (option A)) (a : A) : itree (stmE V) unit :=
-    v <- readTVar t ;;
-    match v with
-    | None => writeTVar t (Some a)
-    | Some _ => retry
-    end.
-
-  Inductive Ty :=
-  | Nat : Ty
-  | Opt : Ty -> Ty.
-
-  Definition Ty_dec (x y : Ty) : {x = y} + {x <> y}.
-    decide equality.
-  Defined.
-
-  #[global] Instance EqDec_Types : EqDec Ty eq := Ty_dec.
-
-  Fixpoint D (type : Ty) : Type :=
-    match type with
-    | Nat => nat
-    | Opt t => option (D t)
-    end.
-
-  Definition message_passing : itree (runStmE D +' forkE) unit :=
-    mv <- atomically (newTVar (Opt Nat) None) ;;
-    done <- atomically (newTVar Nat 0) ;;
-    fork (v1 <- atomically (takeMVar mv) ;; v2 <- atomically (takeMVar mv) ;; atomically (putMVar mv (v1 + v2)))
-         (atomically (putMVar mv 3) ;; atomically (putMVar mv 4) ;; atomically (V := D) (r <- takeMVar mv ;; writeTVar done r)).
-
-  Definition message_passing_simple : itree (runStmE D +' forkE) unit :=
-    mv <- atomically (newTVar (Opt Nat) None) ;;
-    done <- atomically (newTVar Nat 0) ;;
-    fork (v1 <- atomically (takeMVar mv) ;; atomically (putMVar mv (v1 * v1)))
-         (atomically (putMVar mv 3) ;; atomically (V := D) (r <- takeMVar mv ;; writeTVar done r)).
-
-  Definition message_passing_simpler : itree (runStmE D +' forkE) unit :=
-    mv <- atomically (newTVar (Opt Nat) None) ;;
-    done <- atomically (newTVar Nat 0) ;;
-    fork (v1 <- atomically (takeMVar mv) ;; atomically (writeTVar done (v1 * v1)))
-         (atomically (putMVar mv 3)).
-
-  Compute (force 100 (run_atomic_transactions (run_atomically message_passing_simpler))).
-  Compute (force 100 (run_atomic_transactions (run_atomically message_passing_simple))).
-  Compute (force 100 (run_atomic_transactions (run_atomically message_passing))).
-  Compute (force 200 (run_single_lock_fork (run_atomically message_passing_simpler))).
-  Compute (force 200 (run_single_lock_fork (run_atomically message_passing_simple))).
-  Compute (force 300 (run_single_lock_fork (run_atomically message_passing))).
-  Compute (force 1000 (run_tl2_fork (run_atomically message_passing_simpler))).
-  Compute (force 1000 (run_tl2_fork (run_atomically message_passing_simple))).
-  Compute (force 1000 (run_tl2_fork (run_atomically message_passing))).
-
-  (* TODO: tests with orElse *)
-
-End example.
-
-
 
