theories/Monads/STM/Atomic.v
@@ -1,0 +1,21 @@
+From Crane Require Import Monads.ITree.
+
+From ITree Require Import Basics.Basics Basics.CategoryOps.
+
+#[local] Open Scope itree_scope.
+
+Variant atomicE E : Type -> Type :=
+| Atomic : forall {A} (t : itree E A), atomicE E A.
+
+Arguments Atomic {E} {A} (_).
+
+Definition h_atomic {E F} `{E -< F} : atomicE E ~> itree F :=
+  fun _ e =>
+    match e with
+    | Atomic t => translate subevent t
+    end.
+
+Definition run_atomic {E F} `{E -< F} : itree (atomicE E +' F) ~> itree F :=
+  interp (case_ h_atomic (id_ _)).
+
+Arguments run_atomic {E F H T} (t).
