theories/Monads/STM/AtomicTransactions.v
@@ -1,4 +1,4 @@
-From Crane.Monads Require Import ITree STMDefs STM.TransactionDefs STM.ForkDefs STM.WriteLog.
+From Crane.Monads Require Import ITree STMDefs STM.Atomic STM.TransactionDefs STM.ForkDefs STM.WriteLog.
 From Crane.Utils Require Import HMap HAList.
 
 From Stdlib Require Import List Classes.EquivDec.
@@ -11,7 +11,7 @@ Import Basics.Monads.
 
 (* TODO: generalize to any HMap *)
 (* Implements transactions by executing them atomically (blocks all other threads from executing until it is finished) *)
-Definition atomic_transactions {K} {V : K -> Type} `{EqDec K eq}: transactionE (stmE V) ~> atomicE (tvarE V) :=
+Definition h_atomic_transactions {K} {V : K -> Type} `{EqDec K eq}: transactionE (stmE V) ~> atomicE (tvarE V) :=
   fun _ e =>
     match e with
     | Transaction t =>
@@ -26,9 +26,16 @@ Definition atomic_transactions {K} {V : K -> Type} `{EqDec K eq}: transactionE (
                 end)
     end.
 
+Definition atomic_transactions {K} {V : K -> Type} `{EqDec K eq} {E} `{atomicE (tvarE V) -< E}: transactionE (stmE V) ~> itree E :=
+  fun _ e => trigger (h_atomic_transactions _ e).
+
 Definition run_atomic_transactions {K} `{EqDec K eq} {V : K -> Type}
   (t1 : itree (transactionE (stmE V) +' forkE) unit):
   itree void1 (halist (pkey K nat) (pkey_type V) * unit) :=
-  let t2 : itree (atomicE (tvarE V) +' forkE +' tvarE V) unit := translate (bimap atomic_transactions subevent) t1 in
-  let t3 : stateT _ _ _ := interp (handle_tvars _ _) (schedule_rr [t2]) in
-  t3 HMap.empty.
+  let t2 := interp (case_ (C := IFun) (bif := sum1) (c := itree (forkE +' atomicE (tvarE V) +' tvarE V))
+                          atomic_transactions
+                          (fun _ e => trigger e))
+                   t1 in
+  let t3 : itree (tvarE V) unit := run_atomic (schedule_rr [t2]) in
+  let t4 : stateT _ _ _ := interp (handle_tvars _ _) t3 in
+  t4 HMap.empty.
