theories/Monads/STM/Error.v
@@ -1,0 +1,11 @@
+From ITree Require Import ITree Basics.Basics Core.Subevent.
+
+Variant errorE X : Type -> Type :=
+| Error (x : X) : errorE X void.
+
+Arguments Error {X} (x).
+
+Definition error {E X A} `{errorE X -< E} (x : X) : itree E A :=
+  Vis (subevent _ (Error x)) (fun (x : void) => match x with end).
+
+
