theories/Monads/STM/STMTests.v
@@ -1,0 +1,141 @@
+From Crane.Monads Require Import STMDefs.
+From Crane.Monads.STM Require Import
+     ForkDefs
+     TransactionDefs
+     AtomicTransactions
+     SGL
+     TL2.
+
+From ITree Require Import ITree Basics.Basics.
+Import ITreeNotations.
+
+
+From Stdlib Require Import Classes.EquivDec.
+
+Section example.
+
+  #[global] Instance EqDec_unit : EqDec unit eq :=
+    fun x y => match x, y with tt, tt => left eq_refl end.
+
+  Definition nats (_ : unit) : Type := nat.
+
+  Definition fib_trans (x0 x1 : TVar nats nat): itree (stmE nats) unit :=
+    v0 <- readTVar x0 ;;
+    v1 <- readTVar x1 ;;
+    writeTVar x0 v1 ;;
+    writeTVar x1 (v0 + v1).
+
+  Definition fib (n : nat) : itree (runStmE nats +' forkE) unit :=
+    '(x, y) <- atomically (
+      x <- newTVar tt 0 ;;
+      y <- newTVar tt 1 ;;
+      Ret (x, y)) ;;
+    (fix fib_ n :=
+      match n with
+      | 0 => Ret tt
+      | S n => fork (atomically (fib_trans x y)) (fib_ n)
+      end) n.
+
+  Variant result (E : Type -> Type) (A : Type) :=
+  | Val : A -> result E A
+  | NotYet : result E A
+  | Event : forall {X}, E X -> result E A.
+
+  Arguments Val {E A} (a).
+  Arguments NotYet {E A}.
+  Arguments Event {E A} {X} (e).
+
+  Definition force {E A} (n : nat) (t : itree E A) : result E A :=
+    match observe (burn n t) with
+    | RetF a => Val a
+    | TauF _ => NotYet
+    | VisF e _ => Event e
+    end.
+
+  Definition unwrap {E A} : option A -> itree E A :=
+    fun o => match o with None => ITree.spin | Some a => Ret a end.
+
+  Compute (force 200 (run_atomic_transactions (run_atomically (fib 8)))).
+  Compute (force 1000 (run_single_lock_fork (run_atomically (fib 8)))).
+  Compute (force 1874 (run_tl2_fork (run_atomically (fib 8)))).
+
+  Definition read_test : itree (runStmE nats +' forkE) unit :=
+    x <- atomically (newTVar tt 21) ;;
+    atomically (readTVar x) ;;
+    Ret tt.
+
+  Definition write_test : itree (runStmE nats +' forkE) unit :=
+    x <- atomically (newTVar tt 22) ;;
+    atomically (writeTVar x 23).
+
+  Definition inc_test : itree (runStmE nats +' forkE) unit :=
+    x <- atomically (newTVar tt 0) ;;
+    atomically (v <- readTVar x ;; writeTVar x (S v)).
+
+  Compute (force 1000 (run_tl2_fork (run_atomically read_test))).
+  Compute (force 1000 (run_tl2_fork (run_atomically write_test))).
+  Compute (force 1000 (run_tl2_fork (run_atomically inc_test))).
+
+  Definition takeMVar {K} {V : K -> Type} {A} (t : TVar V (option A)) : itree (stmE V) A :=
+    v <- readTVar t ;;
+    match v with
+    | None => retry
+    | Some a => writeTVar t None ;; Ret a
+    end.
+
+  Definition putMVar {K} {V : K -> Type} {A} (t : TVar V (option A)) (a : A) : itree (stmE V) unit :=
+    v <- readTVar t ;;
+    match v with
+    | None => writeTVar t (Some a)
+    | Some _ => retry
+    end.
+
+  Inductive Ty :=
+  | Nat : Ty
+  | Opt : Ty -> Ty.
+
+  Definition Ty_dec (x y : Ty) : {x = y} + {x <> y}.
+    decide equality.
+  Defined.
+
+  #[global] Instance EqDec_Types : EqDec Ty eq := Ty_dec.
+
+  Fixpoint D (type : Ty) : Type :=
+    match type with
+    | Nat => nat
+    | Opt t => option (D t)
+    end.
+
+  Definition message_passing : itree (runStmE D +' forkE) unit :=
+    mv <- atomically (newTVar (Opt Nat) None) ;;
+    done <- atomically (newTVar Nat 0) ;;
+    fork (v1 <- atomically (takeMVar mv) ;; v2 <- atomically (takeMVar mv) ;; atomically (putMVar mv (v1 + v2)))
+         (atomically (putMVar mv 3) ;; atomically (putMVar mv 4) ;; atomically (V := D) (r <- takeMVar mv ;; writeTVar done r)).
+
+  Definition message_passing_simple : itree (runStmE D +' forkE) unit :=
+    mv <- atomically (newTVar (Opt Nat) None) ;;
+    done <- atomically (newTVar Nat 0) ;;
+    fork (v1 <- atomically (takeMVar mv) ;; atomically (putMVar mv (v1 * v1)))
+         (atomically (putMVar mv 3) ;; atomically (V := D) (r <- takeMVar mv ;; writeTVar done r)).
+
+  Definition message_passing_simpler : itree (runStmE D +' forkE) unit :=
+    mv <- atomically (newTVar (Opt Nat) None) ;;
+    done <- atomically (newTVar Nat 0) ;;
+    fork (v1 <- atomically (takeMVar mv) ;; atomically (writeTVar done (v1 * v1)))
+         (atomically (putMVar mv 3)).
+
+  Compute (force 100 (run_atomic_transactions (run_atomically message_passing_simpler))).
+  Compute (force 100 (run_atomic_transactions (run_atomically message_passing_simple))).
+  Compute (force 200 (run_atomic_transactions (run_atomically message_passing))).
+  Compute (force 200 (run_single_lock_fork (run_atomically message_passing_simpler))).
+  Compute (force 200 (run_single_lock_fork (run_atomically message_passing_simple))).
+  Compute (force 300 (run_single_lock_fork (run_atomically message_passing))).
+  Compute (force 1000 (run_tl2_fork (run_atomically message_passing_simpler))).
+  Compute (force 1000 (run_tl2_fork (run_atomically message_passing_simple))).
+  Compute (force 1000 (run_tl2_fork (run_atomically message_passing))).
+
+  (* TODO: tests with orElse *)
+
+End example.
+
+
